Relico.lean
@@ -41,6 +41,7 @@ import Relico.Correctness.Machine
 import Relico.Correctness.MachineInvariant
 import Relico.Correctness.MachineTrace
 import Relico.Correctness.MachineTraceForward
+import Relico.Correctness.MachineInitialization
 import Relico.Correctness.Inversion
 import Relico.Correctness.RuntimeInvariant
 import Relico.Correctness.DispatchInvariant
@@ -70,3 +71,4 @@ import Relico.Tests.MachineCorrectness
 import Relico.Tests.MachineInvariant
 import Relico.Tests.MachineTrace
 import Relico.Tests.MachineTraceForward
+import Relico.Tests.MachineInitialization
